Launchbury/CallFutureCardinality.thy
@@ -1,0 +1,15 @@
+theory CallFutureCardinality
+imports Vars "Cardinality-Domain"
+begin
+
+definition pathCard :: "var list  \<Rightarrow> (var \<Rightarrow> two)"
+  where "pathCard f x = (if x \<notin> set f then none else (if length (filter (\<lambda> y. x = y) f) = 1 then once else many))"
+
+definition pathsCard :: "var list set \<Rightarrow> (var \<Rightarrow> two)"
+  where "pathsCard fs x = lub ((\<lambda> f. pathCard f x)` fs )"
+
+lemma paths_Card_above:
+  "f \<in> fs \<Longrightarrow> pathCard f \<sqsubseteq> pathsCard fs"
+  sorry
+
+end
