Launchbury/FutureCardinality.thy
@@ -1,0 +1,97 @@
+theory FutureCardinality
+imports CallFutures CardinalityAnalysis CallFutureCardinality
+begin
+
+locale FutureAnalysis =
+ fixes Fexp :: "exp \<Rightarrow> Arity \<rightarrow> future set"
+begin
+
+fun FBinds :: "heap \<Rightarrow> AEnv \<rightarrow> (var \<Rightarrow> future set)"
+  where "FBinds [] = (\<Lambda> ae. \<bottom>)"
+      | "FBinds ((x,e)#\<Gamma>) = (\<Lambda> ae. (\<lambda> x'. (if x' = x then fup\<cdot>(Fexp e)\<cdot>(ae x) else (FBinds \<Gamma>\<cdot>ae) x)))"
+
+lemma FBinds_Nil_simp[simp]: "FBinds []\<cdot>ae = \<bottom>" by simp
+
+lemma FBinds_Cons[simp]:
+  "FBinds ((x,e)#\<Gamma>)\<cdot>ae = (\<lambda> x'. (if x' = x then fup\<cdot>(Fexp e)\<cdot>(ae x) else (FBinds \<Gamma>\<cdot>ae) x))" by simp
+
+lemmas FBinds.simps[simp del]
+
+lemma FBinds_cong:
+  assumes "ae f|` domA \<Gamma> = ae' f|` domA \<Gamma>"
+  shows "FBinds \<Gamma>\<cdot>ae = FBinds \<Gamma>\<cdot>ae'"
+using env_restr_eqD[OF assms]
+by (induction \<Gamma> rule: FBinds.induct) (auto split: if_splits)
+
+fun unstack :: "stack \<Rightarrow> exp \<Rightarrow> exp" where
+  "unstack [] e = e"
+| "unstack (Upd x # S) e = unstack S e"
+| "unstack (Arg x # S) e = unstack S (App e x)"
+| "unstack (Dummy x # S) e = unstack S e"
+
+fun Fstack :: "stack \<Rightarrow> future set"
+  where "Fstack [] = \<bottom>"
+  | "Fstack (Upd x # S) = Fstack S"
+  | "Fstack (Arg x # S) = may_call x (Fstack S)"
+  | "Fstack (Dummy x # S) = Fstack S"
+fun prognosis :: "AEnv \<Rightarrow> Arity \<Rightarrow> conf \<Rightarrow> var \<Rightarrow> two"
+   where "prognosis ae a (\<Gamma>, e, S) = pathsCard (paths (FBinds \<Gamma>\<cdot>ae) (future_add (Fexp e\<cdot>a) (Fstack S)))"
+end
+
+locale FutureAnalysisCorrect = FutureAnalysis +
+  assumes Fexp_App: "Fexp (App e x)\<cdot>a = may_call x ((Fexp e)\<cdot>(inc\<cdot>a))"
+begin
+
+
+  sublocale CardinalityPrognosisCorrect prognosis
+  proof
+    fix \<Gamma> :: heap and ae ae' :: AEnv and u e S
+    assume "ae f|` domA \<Gamma> = ae' f|` domA \<Gamma>"
+    from FBinds_cong[OF this]
+    show "prognosis ae u (\<Gamma>, e, S) = prognosis ae' u (\<Gamma>, e, S)" by simp
+  next
+    fix ae a \<Gamma> e S
+    show "const_on (prognosis ae a (\<Gamma>, e, S)) (ap S) many"
+    proof
+      fix x
+      assume "x \<in> ap S"
+      hence "\<exists> f \<in> Fstack S. f x > 1"
+        by(induction S rule: Fstack.induct)(auto simp add: may_call_multiple_calls)
+      hence "\<exists> f \<in> future_add (Fexp e\<cdot>a) (Fstack S). f x > 1"
+        using future_add_subset2 by auto
+      hence "[x,x] \<in> paths (FBinds \<Gamma>\<cdot>ae) (future_add (Fexp e\<cdot>a) (Fstack S))" 
+        apply -
+        apply (erule bexE)
+        apply (rule paths_intros)
+        apply assumption
+        apply (simp add: possible_def)
+        apply (rule paths_intros)
+        apply (rule set_mp[OF future_add_subset1])
+        apply simp
+        apply (simp add: possible_def after_def)
+        apply rule
+        done
+      hence "pathCard [x,x] x \<sqsubseteq> pathsCard (paths (FBinds \<Gamma>\<cdot>ae) (future_add (Fexp e\<cdot>a) (Fstack S))) x"
+        by (metis fun_belowD paths_Card_above)
+      also have "pathCard [x,x] x = many" by (auto simp add: pathCard_def)
+      finally
+      show "prognosis ae a (\<Gamma>, e, S) x = many"
+        by (auto intro: below_antisym)
+    qed
+  next
+    fix ae a \<Gamma> e x S
+    have "future_add (Fexp e\<cdot>(inc\<cdot>a)) (may_call x (Fstack S)) = future_add (may_call x (Fexp e\<cdot>(inc\<cdot>a))) (Fstack S)"
+      by (rule future_add_may_call_twist)
+    hence "(future_add (Fexp e\<cdot>(inc\<cdot>a)) (may_call x (Fstack S))) = future_add (Fexp (App e x)\<cdot>a) (Fstack S)"
+      by (simp add: Fexp_App)
+    thus "prognosis ae (inc\<cdot>a) (\<Gamma>, e, Arg x # S) \<sqsubseteq> prognosis ae a (\<Gamma>, App e x, S)"
+      by simp
+  next
+  oops
+
+end
+
+
+
+end
+  
